src/Iris/Algebra/Heap.lean
@@ -82,7 +82,7 @@ open PartialMap
 
 variable [LawfulPartialMap M K] [CMRA V]
 
-@[simp] def op (s1 s2 : M V) : M V := merge (K := K) (fun _ => CMRA.op) s1 s2
+@[simp] def op (s1 s2 : M V) : M V := merge (fun _ => CMRA.op) s1 s2
 @[simp] def unit : M V := empty
 @[simp] def pcore (s : M V) : Option (M V) := some <| bindAlter (fun _ => CMRA.pcore) s
 @[simp] def valid (s : M V) : Prop := ∀ k, ✓ get? s k
